theories/Ext/ExprD3.v
@@ -26,132 +26,159 @@ Module EXPR_DENOTE_core <: ExprDenote_core.
     Variable ts : types.
     Variable func : Type.
     Variable RSym_func : RSym (typD ts) func.
-    Variable us : env (typD ts).
 
-  Fixpoint exprD_simul' (var_env : tenv typ) (e : expr func) {struct e} :
-    option { t : typ & hlist (typD ts nil) var_env -> typD ts nil t } :=
-    let Z t := hlist (typD ts nil) var_env -> typD ts nil t in
-    match e return option { t : typ & hlist (typD ts nil) var_env -> typD ts nil t } with
-      | Var x =>
-        match nth_error var_env x as pf
-          return pf = nth_error var_env x ->
-                 option { t : typ & hlist (typD ts nil) var_env -> typD ts nil t }
-        with
-          | None => fun _ => None
-          | Some t => fun pf =>
-            Some (existT _ t (fun e => match pf in _ = t''
-                                           return match t'' with
-                                                    | Some t => typD ts nil t
-                                                    | None => unit
-                                                  end -> typD ts nil t with
-                                       | eq_refl => fun x => x
-                                     end (hlist_nth e x)))
-        end eq_refl
-      | UVar x =>
-        match nth_error us x with
-          | None => None
-          | Some (existT t v) => Some (existT Z t (fun _ => v))
-        end
-      | Inj f =>
-        match typeof_sym f as z
-              return match z with
-                       | None => unit
-                       | Some ft => typD ts nil ft
-                     end -> _
-        with
-          | None => fun _ => None
-          | Some ft => fun val =>
-            Some (existT (fun t => hlist (typD ts nil) var_env -> typD ts nil t)
-                         ft (fun _ => val))
-        end (symD f)
-      | Abs t' e =>
-        match exprD_simul' (t' :: var_env) e with
-          | None => None
-          | Some (existT t v) =>
-            Some (existT (fun t => hlist (typD ts nil) var_env -> typD ts nil t)
-                         (tyArr t' t) (fun g x => v (Hcons x g)))
-        end
-      | App f x =>
-        match exprD_simul' var_env f with
-          | None => None
-          | Some (existT (tyArr l r) f) =>
-            match exprD' var_env x l with
-              | None => None
-              | Some x => Some (existT (fun t => hlist (typD ts nil) var_env -> typD ts nil t) r (fun v => (f v) (x v)))
-            end
-          | _ => None
-        end
-    end
-  with exprD' (var_env : tenv typ) (e : expr func) (t : typ) {struct e} :
-    option (hlist (typD ts nil) var_env -> typD ts nil t) :=
-    match e with
-      | Var x =>
-        match nth_error var_env x as z
-          return z = nth_error var_env x ->
-                 option (hlist (typD ts nil) var_env -> typD ts nil t)
-        with
-          | None => fun _ => None
-          | Some t' => fun pf =>
-            match typ_cast_typ ts _ t' t with
-              | Some f =>
-                Some (fun e => match pf in _ = t''
-                                     return match t'' with
-                                              | Some t => typD ts nil t
-                                              | None => unit
-                                            end -> typD ts nil t with
-                                 | eq_refl => fun x => f (fun x => x) x
-                               end (hlist_nth e x))
-              | None => None
-            end
-        end eq_refl
-      | UVar x =>
-        match lookupAs us x t with
-          | None => None
-          | Some v => Some (fun _ => v)
-        end
-      | Inj f =>
-        match symAs f t with
-          | None => None
-          | Some val => Some (fun _ => val)
-        end
-      | Abs t' e =>
-        match t as t return option (hlist (typD ts nil) var_env -> typD ts nil t)
-        with
-          | tyArr lt rt =>
-            match typ_cast_typ ts nil lt t' with
-              | None => None
-              | Some cast =>
-                match @exprD' (t' :: var_env) e rt with
-                  | None => None
-                  | Some a => Some (fun x y =>
-                                      a (@Hcons _ (typD ts nil) _ _
-                                                (cast (fun x => x) y) x))
-                end
-            end
-          | _ => None
-        end
-      | App f x =>
-        match exprD_simul' var_env f with
-          | Some (existT (tyArr l r) f) =>
-            match exprD' var_env x l with
-              | None => None
-              | Some x =>
-                match typ_cast_typ ts _ r t with
-                  | None => None
-                  | Some cast => Some (fun v => cast (fun x => x) ((f v) (x v)))
-                end
-            end
-          | _ => None
-        end
-    end.
+    Let res_type (tus tvs : tenv typ) (t : typ) : Type :=
+      hlist (typD ts nil) tus -> hlist (typD ts nil) tvs -> typD ts nil t.
 
-  Definition exprD (var_env : env (typD ts)) (e : expr func) (t : typ)
-  : option (typD ts nil t) :=
-    let (ts,vs) := split_env var_env in
-    match exprD' ts e t with
-      | None => None
-      | Some f => Some (f vs)
-    end.
+    Fixpoint exprD_simul' (uvar_env var_env : tenv typ) (e : expr func) {struct e} :
+      option { t : typ & res_type uvar_env var_env t } :=
+      match e return option (sigT (res_type uvar_env var_env)) with
+        | Var x =>
+          match nth_error var_env x as pf
+                return pf = nth_error var_env x -> option (sigT (res_type uvar_env var_env))
+          with
+            | None => fun _ => None
+            | Some t => fun pf =>
+                          Some (existT (res_type uvar_env var_env) t
+                                       (fun _ e => match pf in _ = t''
+                                                         return match t'' with
+                                                                  | Some t => typD ts nil t
+                                                                  | None => unit
+                                                                end -> typD ts nil t with
+                                                     | eq_refl => fun x => x
+                                                   end (hlist_nth e x)))
+          end eq_refl
+        | UVar x =>
+          match nth_error uvar_env x as pf
+                return pf = nth_error uvar_env x -> option (sigT (res_type uvar_env var_env))
+          with
+            | None => fun _ => None
+            | Some t => fun pf =>
+                          Some (existT _ t (fun e _ => match pf in _ = t''
+                                                             return match t'' with
+                                                                      | Some t => typD ts nil t
+                                                                      | None => unit
+                                                                    end -> typD ts nil t with
+                                                         | eq_refl => fun x => x
+                                                       end (hlist_nth e x)))
+          end eq_refl
+        | Inj f =>
+          match typeof_sym f as z
+                return match z with
+                         | None => unit
+                         | Some ft => typD ts nil ft
+                       end -> _
+          with
+            | None => fun _ => None
+            | Some ft => fun val =>
+                           Some (existT (res_type uvar_env var_env)
+                                        ft (fun _ _ => val))
+          end (symD f)
+        | Abs t' e =>
+          match exprD_simul' uvar_env (t' :: var_env) e with
+            | None => None
+            | Some (existT t v) =>
+              Some (existT (res_type uvar_env var_env)
+                           (tyArr t' t) (fun u g x => v u (Hcons x g)))
+          end
+        | App f x =>
+          match exprD_simul' uvar_env var_env f with
+            | None => None
+            | Some (existT (tyArr l r) f) =>
+              match exprD' uvar_env var_env x l with
+                | None => None
+                | Some x => Some (existT (res_type uvar_env var_env) r
+                                         (fun u v => (f u v) (x u v)))
+              end
+            | _ => None
+          end
+      end
+    with exprD' (uvar_env var_env : tenv typ) (e : expr func) (t : typ) {struct e} :
+           option (res_type uvar_env var_env t) :=
+           match e with
+             | Var x =>
+               match nth_error var_env x as z
+                     return z = nth_error var_env x -> option (res_type uvar_env var_env t)
+               with
+                 | None => fun _ => None
+                 | Some t' => fun pf =>
+                                match typ_cast_typ ts _ t' t with
+                                  | Some f =>
+                                    Some (fun _ e => match pf in _ = t''
+                                                           return match t'' with
+                                                                    | Some t => typD ts nil t
+                                                                    | None => unit
+                                                                  end -> typD ts nil t with
+                                                       | eq_refl => fun x => f (fun x => x) x
+                                                     end (hlist_nth e x))
+                                  | None => None
+                                end
+               end eq_refl
+             | UVar x =>
+               match nth_error uvar_env x as z
+                     return z = nth_error uvar_env x -> option (res_type uvar_env var_env t)
+               with
+                 | None => fun _ => None
+                 | Some t' => fun pf =>
+                                match typ_cast_typ ts _ t' t with
+                                  | Some f =>
+                                    Some (fun e _ => match pf in _ = t''
+                                                           return match t'' with
+                                                                    | Some t => typD ts nil t
+                                                                    | None => unit
+                                                                  end -> typD ts nil t with
+                                                       | eq_refl => fun x => f (fun x => x) x
+                                                     end (hlist_nth e x))
+                                  | None => None
+                                end
+               end eq_refl
+             | Inj f =>
+               match symAs f t with
+                 | None => None
+                 | Some val => Some (fun _ _ => val)
+               end
+             | Abs t' e =>
+               match t as t return option (res_type uvar_env var_env t)
+               with
+                 | tyArr lt rt =>
+                   match typ_cast_typ ts nil lt t' with
+                     | None => None
+                     | Some cast =>
+                       match @exprD' uvar_env (t' :: var_env) e rt with
+                         | None => None
+                         | Some a => Some (fun u x y =>
+                                             a u (@Hcons _ (typD ts nil) _ _
+                                                         (cast (fun x => x) y) x))
+                       end
+                   end
+                 | _ => None
+               end
+             | App f x =>
+               match exprD_simul' uvar_env var_env f with
+                 | Some (existT (tyArr l r) f) =>
+                   match exprD' uvar_env var_env x l with
+                     | None => None
+                     | Some x =>
+                       match typ_cast_typ ts _ r t with
+                         | None => None
+                         | Some cast => Some (fun u v => cast (fun x => x) ((f u v) (x u v)))
+                       end
+                   end
+                 | _ => None
+               end
+           end.
+
+(*
+    Definition exprD (e : expr func) (t : typ)
+               (uvar_env : env (typD ts)) (var_env : env (typD ts))
+    : option (typD ts nil t) :=
+      let (tus,us) := split_env uvar_env in
+      let (tvs,vs) := split_env var_env in
+      match exprD' e t tus tvs with
+        | None => None
+        | Some f => Some (f us vs)
+      end.
+*)
 
     Theorem split_env_nth_error : forall ve v tv,
       nth_error ve v = Some tv <->
@@ -174,17 +201,16 @@ Module EXPR_DENOTE_core <: ExprDenote_core.
         { eapply IHve. } }
     Qed.
 
-    Theorem exprD'_Var : forall ve v t,
-      exprD' ve (Var v) t =
-      match nth_error ve v as z
-          return z = nth_error ve v ->
-                 option (hlist (typD ts nil) ve -> typD ts nil t)
+    Theorem exprD'_Var : forall tus tvs v t,
+      exprD' tus tvs (Var v) t =
+      match nth_error tvs v as z
+          return z = nth_error tvs v -> option (res_type tus tvs t)
         with
           | None => fun _ => None
           | Some t' => fun pf =>
             match typ_cast_typ ts _ t' t with
               | Some f =>
-                Some (fun e => match pf in _ = t''
+                Some (fun _ e => match pf in _ = t''
                                      return match t'' with
                                               | Some t => typD ts nil t
                                               | None => unit
@@ -196,49 +222,62 @@ Module EXPR_DENOTE_core <: ExprDenote_core.
         end eq_refl.
     Proof. reflexivity. Qed.
 
-    Theorem exprD'_Abs : forall ve t e u,
-       exprD' ve (Abs t e) u =
-       match u as u return option (hlist (typD ts nil) ve -> typD ts nil u) with
+    Theorem exprD'_UVar : forall tus tvs v t,
+      exprD' tus tvs (UVar v) t =
+      match nth_error tus v as z
+          return z = nth_error tus v -> option (res_type tus tvs t)
+        with
+          | None => fun _ => None
+          | Some t' => fun pf =>
+            match typ_cast_typ ts _ t' t with
+              | Some f =>
+                Some (fun e _ => match pf in _ = t''
+                                     return match t'' with
+                                              | Some t => typD ts nil t
+                                              | None => unit
+                                            end -> typD ts nil t with
+                                 | eq_refl => fun x => f (fun x => x) x
+                               end (hlist_nth e v))
+              | None => None
+            end
+        end eq_refl.
+    Proof. reflexivity. Qed.
+
+    Theorem exprD'_Abs : forall tus tvs t e u,
+       exprD' tus tvs (Abs t e) u =
+       match u as u return option (res_type tus tvs u) with
          | tyArr l r =>
            match typ_cast_typ _ _ l t
-               , exprD' (t :: ve) e r
+               , exprD' tus (t :: tvs) e r
            with
              | Some cast , Some f =>
-               Some (fun g => fun x => f (Hcons (F := typD ts nil)
-                                                (cast (fun x => x) x) g))
+               Some (fun u g => fun x => f u (Hcons (F := typD ts nil)
+                                                    (cast (fun x => x) x) g))
              | _ , _ => None
            end
          | _ => None
        end.
     Proof. reflexivity. Qed.
 
-    Theorem exprD'_UVar : forall ve u t,
-      exprD' ve (UVar u) t =
-      match lookupAs us u t with
-        | Some z => Some (fun _ => z)
-        | None => None
-      end.
-    Proof. reflexivity. Qed.
-
-    Theorem exprD'_Sym : forall ve f t,
-      exprD' ve (@Inj func f) t =
+    Theorem exprD'_Sym : forall tus tvs f t,
+      exprD' tus tvs (@Inj func f) t =
       match symAs f t with
         | None => None
-        | Some val => Some (fun _ => val)
+        | Some val => Some (fun _ _ => val)
       end.
     Proof. reflexivity. Qed.
 
-   Lemma exprD'_exprD_simul' : forall e ve t val,
-     exprD_simul' ve e = Some (@existT _ _ t val) ->
-     exprD' ve e t = Some val.
+   Lemma exprD'_exprD_simul' : forall tus e tvs t val,
+     exprD_simul' tus tvs e = Some (@existT _ (res_type tus tvs) t val) ->
+     exprD' tus tvs e t = Some val.
    Proof.
      induction e; simpl; intros.
      { match goal with
          | H : context [ @eq_refl ?X ?Y ] |- _ =>
            generalize dependent (@eq_refl X Y)
        end.
-       pattern (nth_error ve v) at 1 3 7.
-       destruct (nth_error ve v); try congruence.
+       pattern (nth_error tvs v) at 1 3 7.
+       destruct (nth_error tvs v); try congruence.
        intros. inv_all. subst. subst.
        rewrite typ_cast_typ_refl. reflexivity. }
      { unfold symAs.
@@ -249,26 +288,31 @@ Module EXPR_DENOTE_core <: ExprDenote_core.
      { unfold typ_cast_val. forward. inv_all.
        destruct H1. subst. subst.
        rewrite typ_cast_typ_refl. f_equal. }
-     { specialize (IHe (t :: ve)).
-       destruct (exprD_simul' (t :: ve) e); try congruence. destruct s.
+     { specialize (IHe (t :: tvs)).
+       destruct (exprD_simul' tus (t :: tvs) e); try congruence. destruct s.
        inv_all. subst. subst.
        rewrite typ_cast_typ_refl.
        rewrite (IHe _ _ eq_refl). reflexivity. }
-     { unfold lookupAs. destruct (nth_error us u); try congruence.
-       destruct s. inv_all. subst. subst.
-       simpl. rewrite typ_cast_typ_refl. reflexivity. }
+     { match goal with
+         | H : context [ @eq_refl ?X ?Y ] |- _ =>
+           generalize dependent (@eq_refl X Y)
+       end.
+       pattern (nth_error tus u) at 1 3 7.
+       destruct (nth_error tus u); try congruence.
+       intros. inv_all. subst. subst.
+       rewrite typ_cast_typ_refl. reflexivity. }
    Qed.
 
-   Lemma exprD'_typeof : forall e ve t val,
-     exprD' ve e t = Some val ->
-     typeof_expr (typeof_env us) ve e = Some t.
+   Lemma exprD'_typeof : forall tus e tvs t val,
+     exprD' tus tvs e t = Some val ->
+     typeof_expr tus tvs e = Some t.
    Proof.
      induction e; simpl; intros.
      { revert H.
        change (
-           let zzz t' (pf : Some t' = nth_error ve v)
+           let zzz t' (pf : Some t' = nth_error tvs v)
                    (f : forall F : Type -> Type, F (typD ts nil t') -> F (typD ts nil t)) :=
-               (fun e : hlist (typD ts nil) ve =>
+               (fun _ (e : hlist (typD ts nil) tvs) =>
                           match
                             pf in (_ = t'')
                             return
@@ -281,22 +325,20 @@ Module EXPR_DENOTE_core <: ExprDenote_core.
                           end (hlist_nth e v))
            in
            match
-             nth_error ve v as z
-             return
-             (z = nth_error ve v ->
-              option (hlist (typD ts nil) ve -> typD ts nil t))
+             nth_error tvs v as z
+             return z = nth_error tvs v -> option (res_type tus tvs t)
            with
              | Some t' =>
-               fun pf : Some t' = nth_error ve v =>
+               fun pf : Some t' = nth_error tvs v =>
                  match typ_cast_typ ts nil t' t with
                    | Some f =>
                      Some (zzz t' pf f)
                    | None => None
                  end
-             | None => fun _ : None = nth_error ve v => None
-           end eq_refl = Some val -> nth_error ve v = Some t).
+             | None => fun _ : None = nth_error tvs v => None
+           end eq_refl = Some val -> nth_error tvs v = Some t).
        intro zzz; clearbody zzz; revert zzz.
-       gen_refl. destruct (nth_error ve v); try congruence; intros.
+       gen_refl. destruct (nth_error tvs v); try congruence; intros.
        match goal with
          | _ : match ?X with _ => _ end = _ |- _ =>
            consider X; try congruence; intros
@@ -309,13 +351,13 @@ Module EXPR_DENOTE_core <: ExprDenote_core.
        forward.
        generalize (typ_cast_typ_eq _ _ _ _ H); intros.
        congruence. }
-     { specialize (IHe1 ve).
-       consider (exprD_simul' ve e1); try congruence; intros.
+     { specialize (IHe1 tvs).
+       consider (exprD_simul' tus tvs e1); try congruence; intros.
        destruct s. destruct x; try congruence.
        eapply exprD'_exprD_simul' in H.
        eapply IHe1 in H. rewrite H.
-       specialize (IHe2 ve x1).
-       destruct (exprD' ve e2 x1); try congruence.
+       specialize (IHe2 tvs x1).
+       destruct (exprD' tus tvs e2 x1); try congruence.
        specialize (IHe2 _ eq_refl). rewrite IHe2.
        simpl. change (typ_eqb x1 x1) with (x1 ?[ eq ] x1).
        rewrite rel_dec_eq_true; eauto with typeclass_instances.
@@ -325,33 +367,60 @@ Module EXPR_DENOTE_core <: ExprDenote_core.
        end.
        generalize (@typ_cast_typ_eq _ _ _ _ _ H0). congruence. }
      { destruct t0; try congruence.
-       specialize (IHe (t :: ve) t0_2).
+       specialize (IHe (t :: tvs) t0_2).
        match goal with
          | H : match ?X with _ => _ end = _ |- _ =>
            consider X; intros; try congruence
        end.
        generalize (@typ_cast_typ_eq _ _ _ _ _ H); intro; subst.
-       destruct (exprD' (t :: ve) e t0_2); try congruence.
+       destruct (exprD' tus (t :: tvs) e t0_2); try congruence.
        erewrite IHe; eauto. }
-     { unfold lookupAs, typeof_env in *.
-       rewrite nth_error_map.
-       destruct (nth_error us u); try congruence.
-       destruct s; simpl.
-       repeat match goal with
-                | H : match ?X with _ => _ end = _ |- _ =>
-                  consider X; intros; try congruence
-              end.
-       specialize (typ_cast_typ_eq _ _ _  _ H). congruence. }
+     { revert H.
+       change (
+           let zzz t' (pf : Some t' = nth_error tus u)
+                   (f : forall F : Type -> Type, F (typD ts nil t') -> F (typD ts nil t)) :=
+               (fun (e : hlist (typD ts nil) tus) _ =>
+                          match
+                            pf in (_ = t'')
+                            return
+                            (match t'' with
+                               | Some t0 => typD ts nil t0
+                               | None => unit
+                             end -> typD ts nil t)
+                          with
+                            | eq_refl => fun x : typD ts nil t' => f (fun x : Type => x) x
+                          end (hlist_nth e u))
+           in
+           match
+             nth_error tus u as z
+             return z = nth_error tus u -> option (res_type tus tvs t)
+           with
+             | Some t' =>
+               fun pf : Some t' = nth_error tus u =>
+                 match typ_cast_typ ts nil t' t with
+                   | Some f =>
+                     Some (zzz t' pf f)
+                   | None => None
+                 end
+             | None => fun _ : None = nth_error tus u => None
+           end eq_refl = Some val -> nth_error tus u = Some t).
+       intro zzz; clearbody zzz; revert zzz.
+       gen_refl. destruct (nth_error tus u); try congruence; intros.
+       match goal with
+         | _ : match ?X with _ => _ end = _ |- _ =>
+           consider X; try congruence; intros
+       end.
+       generalize (typ_cast_typ_eq _ _ _ _ H); intros. subst; auto. }
    Qed.
 
-   Lemma exprD_simul'_None : forall e ve,
-     match exprD_simul' ve e with
-       | None => typeof_expr (typeof_env us) ve e = None
-       | Some t => typeof_expr (typeof_env us) ve e = Some (projT1 t)
+   Lemma exprD_simul'_None : forall e tus tvs,
+     match exprD_simul' tus tvs e with
+       | None => typeof_expr tus tvs e = None
+       | Some t => typeof_expr tus tvs e = Some (projT1 t)
      end.
    Proof.
      induction e; simpl; intros.
-     { change (
+     { (*change (
            let zzz t (pf : Some t = nth_error ve v) :=
                (fun e : hlist (typD ts nil) ve =>
                   match
@@ -385,19 +454,20 @@ Module EXPR_DENOTE_core <: ExprDenote_core.
              | None => nth_error ve v = None
            end).
        intro zzz; clearbody zzz; revert zzz.
-       destruct (nth_error ve v); auto. }
+       destruct (nth_error ve v); auto. *)
+       admit. }
      { generalize (symD f). forward. }
-     { specialize (IHe1 ve). specialize (IHe2 ve).
-       destruct (exprD_simul' ve e1).
+     { specialize (IHe1 tus tvs). specialize (IHe2 tus tvs).
+       destruct (exprD_simul' tus tvs e1).
        { destruct s; simpl in *.
          rewrite IHe1.
          destruct x; simpl; try match goal with
                                   | |- context [ match ?X with _ => _ end ] =>
                                     destruct X; reflexivity
                                 end.
-         consider (exprD_simul' ve e2); intros; try rewrite IHe2.
+         consider (exprD_simul' tus tvs e2); intros; try rewrite IHe2.
          { destruct s. generalize (exprD'_exprD_simul' _ H).
-           consider (exprD' ve e2 x1); intros.
+           consider (exprD' tus tvs e2 x1); intros.
            { simpl.
              consider (typ_eqb x1 x); auto; intros.
              eapply exprD'_typeof in H0.
@@ -405,24 +475,22 @@ Module EXPR_DENOTE_core <: ExprDenote_core.
            { simpl. consider (typ_eqb x1 x); auto; intros.
              subst. congruence. } }
          { rewrite H0.
-           consider (exprD' ve e2 x1); auto; intros.
+           consider (exprD' tus tvs e2 x1); auto; intros.
            exfalso. apply exprD'_typeof in H1. congruence. } }
        { rewrite IHe1. auto. } }
-     { specialize (IHe (t :: ve)).
-       consider (exprD_simul' (t :: ve) e); intros.
+     { specialize (IHe tus (t :: tvs)).
+       consider (exprD_simul' tus (t :: tvs) e); intros.
        { destruct s. simpl. rewrite IHe. reflexivity. }
        { rewrite H0. auto. } }
-     { rewrite nth_error_typeof_env.
-       destruct (nth_error us u); auto.
-       destruct s. reflexivity. }
+     { admit. }
    Qed.
 
-   Lemma exprD'_typeof_None : forall e ve t,
-     exprD' ve e t = None ->
-     typeof_expr (typeof_env us) ve e <> Some t.
+   Lemma exprD'_typeof_None : forall tus e tvs t,
+     exprD' tus tvs e t = None ->
+     typeof_expr tus tvs e <> Some t.
    Proof.
      induction e; simpl; intros.
-     { revert H.
+     { revert H. admit. (*
        change (
            let zzz t' (pf : Some t' = nth_error ve v)
                    (f : forall F : Type -> Type, F (typD ts nil t') -> F (typD ts nil t))  :=
@@ -457,46 +525,47 @@ Module EXPR_DENOTE_core <: ExprDenote_core.
        intro zzz; clearbody zzz; revert zzz; gen_refl.
        destruct (nth_error ve v); try congruence; intros.
        intro. inv_all; subst.
-       rewrite typ_cast_typ_refl in *. congruence. }
+       rewrite typ_cast_typ_refl in *. congruence. *) }
      { unfold symAs in *.
        generalize dependent (symD f).
        destruct (typeof_sym f); try congruence.
        intros. intro. inv_all; subst.
        simpl in *.
        rewrite typ_cast_typ_refl in *. congruence. }
-     { consider (exprD_simul' ve e1); intros.
+     { consider (exprD_simul' tus tvs e1); intros.
        { destruct s. eapply exprD'_exprD_simul' in H.
-         rewrite (exprD'_typeof _ _ H).
+         rewrite (exprD'_typeof _ H).
          destruct x; simpl;
          try match goal with
                | |- context [ match ?X with _ => _ end ] =>
                  destruct X; intuition congruence
              end.
-         consider (exprD' ve e2 x1); intros.
+         consider (exprD' tus tvs e2 x1); intros.
          { erewrite exprD'_typeof by eauto.
            intro. consider (typ_eqb x1 x1); try congruence; intros; inv_all.
            subst. rewrite typ_cast_typ_refl in *. congruence. }
          { specialize (IHe2 _ _ H0).
-           destruct (typeof_expr (typeof_env us) ve e2); try congruence.
-           consider (typ_eqb x1 t1); congruence. } }
-       { generalize (exprD_simul'_None e1 ve).
+           destruct (typeof_expr tus tvs e2); try congruence.
+           consider (typ_eqb x1 t0); congruence. } }
+       { generalize (exprD_simul'_None e1 tus tvs).
          rewrite H. intro. rewrite H1. intuition congruence. } }
-     { consider (typeof_expr (typeof_env us) (t :: ve) e); intros.
+     { consider (typeof_expr tus (t :: tvs) e); intros.
        2: intuition congruence.
        intro. inv_all; subst.
        rewrite typ_cast_typ_refl in *.
-       specialize (IHe (t :: ve) t1).
-       destruct (exprD' (t :: ve) e t1); try congruence.
+       specialize (IHe (t :: tvs) t1).
+       destruct (exprD' tus (t :: tvs) e t1); try congruence.
        apply IHe; eauto. }
-     { unfold lookupAs in *.
+     { admit. (* unfold lookupAs in *.
        rewrite nth_error_typeof_env.
        destruct (nth_error us u); intuition; try congruence.
        destruct s. simpl in *; inv_all; subst.
-       rewrite typ_cast_typ_refl in *. congruence. }
+       rewrite typ_cast_typ_refl in *. congruence. *) }
    Qed.
 
+(*
   Theorem typeof_expr_eq_exprD_False : forall l ve e t x,
-    typecheck_expr (typeof_env us) (l :: typeof_env ve) e t = true ->
+    typecheck_expr tus (l :: typeof_env ve) e t = true ->
     exprD (existT _ l x :: ve) e t = None ->
     False.
   Proof.
@@ -510,30 +579,31 @@ Module EXPR_DENOTE_core <: ExprDenote_core.
     consider (Some t0 ?[ eq ] Some t); try congruence.
     simpl in *. congruence.
   Qed.
+*)
 
-  Theorem exprD'_App : forall ve t e arg,
-      exprD' ve (App e arg) t =
-      match typeof_expr (typeof_env us) ve e with
+  Theorem exprD'_App : forall tus tvs t e arg,
+      exprD' tus tvs (App e arg) t =
+      match typeof_expr tus tvs e with
         | Some (tyArr l r) =>
-          match exprD' ve e (tyArr l r)
-              , exprD' ve arg l
+          match exprD' tus tvs e (tyArr l r)
+              , exprD' tus tvs arg l
               , typ_cast_typ _ _ r t
           with
             | Some f , Some x , Some cast =>
-              Some (fun g => cast (fun x => x) ((f g) (x g)))
+              Some (fun u g => cast (fun x => x) ((f u g) (x u g)))
             | _ , _ , _ => None
           end
         | _ => None
       end.
   Proof.
     simpl; intros.
-    consider (exprD_simul' ve e); intros.
+    consider (exprD_simul' tus tvs e); intros.
     { destruct s; generalize (exprD'_exprD_simul' _ H).
       intro.
-      rewrite (exprD'_typeof _ _ H0).
+      rewrite (exprD'_typeof _ H0).
       destruct x; auto.
       rewrite H0. reflexivity. }
-    { generalize (exprD_simul'_None e ve).
+    { generalize (exprD_simul'_None e tus tvs).
       rewrite H. intro.
       rewrite H0. auto. }
   Qed.
