theories/ExprSem.v
@@ -1,0 +1,105 @@
+Require Import RelationClasses.
+Require Import Morphisms Relations.
+Require Import ExtLib.Data.HList.
+Require Import MirrorCore.SymI.
+Require Import MirrorCore.EnvI.
+Require Import MirrorCore.ExprI.
+
+Set Implicit Arguments.
+Set Strict Implicit.
+
+Section sem.
+  Variable typ : Type.
+  Variable typD : list Type -> typ -> Type.
+  Variable expr : Type.
+  Variable Expr_expr : Expr typD expr.
+
+  Definition Sem_equiv' (t : typ) (R : relation (typD nil t)) (tus tvs : tenv typ)
+  : relation expr :=
+    fun x y =>
+        match exprD' tus tvs x t , exprD' tus tvs y t with
+          | None , None => True
+          | Some l , Some r =>
+            forall us vs, R (l us vs) (r us vs)
+          | _ , _ => False
+        end.
+
+  Instance Reflexive_Sem_equiv' t Rt (Refl_Rt : Reflexive Rt) tus tvs
+  : Reflexive (@Sem_equiv' t Rt tus tvs).
+  Proof.
+    red. red; intros. destruct (exprD' tus tvs x t); auto.
+  Qed.
+
+  Instance Symmetric_Sem_equiv' t Rt (Refl_Rt : Symmetric Rt) tus tvs
+  : Symmetric (@Sem_equiv' t Rt tus tvs).
+  Proof.
+    red. unfold Sem_equiv'. intros.
+    destruct (exprD' tus tvs x t);
+    destruct (exprD' tus tvs y t); intuition.
+  Qed.
+
+  Instance Transitive_Sem_equiv' t Rt (Refl_Rt : Transitive Rt) tus tvs
+  : Transitive (@Sem_equiv' t Rt tus tvs).
+  Proof.
+    red. unfold Sem_equiv'; simpl; intros.
+    destruct (exprD' tus tvs x t);
+      destruct (exprD' tus tvs y t);
+      destruct (exprD' tus tvs z t); auto.
+    { intros. etransitivity. eapply H. eauto. }
+    { intuition. }
+  Qed.
+
+  Definition Sem_equiv (t : typ) (R : relation (typD nil t)) (us vs : env (typD))
+  : relation expr :=
+    fun x y =>
+      match exprD us vs x t , exprD us vs y t with
+        | None , None => True
+        | Some l , Some r => R l r
+        | _ , _ => False
+      end.
+
+  Instance Reflexive_Sem_equiv t Rt (Refl_Rt : Reflexive Rt) us vs
+  : Reflexive (@Sem_equiv t Rt us vs).
+  Proof.
+    red. red; intros.
+    destruct (exprD us vs x t); auto.
+  Qed.
+
+  Instance Symmetric_Sem_equiv t Rt (Refl_Rt : Symmetric Rt) us vs
+  : Symmetric (@Sem_equiv t Rt us vs).
+  Proof.
+    red. unfold Sem_equiv. intros.
+    destruct (exprD us vs x t);
+    destruct (exprD us vs y t); intuition.
+  Qed.
+
+  Instance Transitive_Sem_equiv t Rt (Refl_Rt : Transitive Rt) us vs
+  : Transitive (@Sem_equiv t Rt us vs).
+  Proof.
+    red. unfold Sem_equiv.
+    intros.
+    destruct (exprD us vs x t);
+      destruct (exprD us vs y t);
+      destruct (exprD us vs z t); auto.
+    { intros. etransitivity. eapply H. eauto. }
+    { intuition. }
+  Qed.
+
+  Definition Sem_ext (t : typ) (P : typD nil t -> Prop) (Q : Prop) us vs
+  : expr -> Prop :=
+    fun e =>
+      match exprD us vs e t with
+        | Some val => P val
+        | None => Q
+      end.
+
+  Definition Sem_ext' (t : typ) (P : typD nil t -> Prop) (Q : Prop) tus tvs
+  : expr -> Prop :=
+    fun e =>
+        match exprD' tus tvs e t with
+          | Some val =>
+            forall us vs, P (val us vs)
+          | None => Q
+        end.
+
+End sem.
