theories/Ext/Expr.v
@@ -1,3 +1,5 @@
+Require Export MirrorCore.ExprI.
+Require Export MirrorCore.SymI.
 Require Export MirrorCore.Ext.Types.
 Require Export MirrorCore.Ext.ExprCore.
 Require Export MirrorCore.Ext.ExprD.
@@ -5,6 +7,3 @@ Require Export MirrorCore.Ext.ExprT.
 Require Export MirrorCore.Ext.ExprFacts.
 Require Export MirrorCore.Ext.ExprLift.
 Require Export MirrorCore.Ext.ExprTactics.
-(*
-Require Export MirrorCore.Ext.ExprSubst.
-*)
