theories/Ext/LemmaExt.v
@@ -20,16 +20,16 @@ Section with_expr.
   Variable ts : types.
   Variable func : Type.
   Variable conclusion : Type.
-  Variable conclusionD : env (typD ts) -> forall vs : list typ,
-                                            conclusion ->
-                                            option (hlist (typD ts nil) vs -> Prop).
+  Variable conclusionD : forall us vs : list typ,
+                           conclusion ->
+                           option (hlist (typD ts nil) us -> hlist (typD ts nil) vs -> Prop).
   Hypothesis conclusionD_weaken : forall us tvs c val,
     conclusionD us tvs c = Some val ->
     forall us' tvs',
       exists val',
         conclusionD (us ++ us') (tvs ++ tvs') c = Some val' /\
-        forall x y,
-          val x = val' (hlist_app x y).
+        forall u u' x y,
+          val u x = val' (hlist_app u u') (hlist_app x y).
 
   Record lemma : Type :=
   { vars : list typ
@@ -83,17 +83,18 @@ Section with_expr.
 
   Definition lemmaD (us vs : env (typD ts)) (l : lemma) : Prop :=
     let (tvs,vs) := split_env vs in
+    let (tus,us) := split_env us in
     match mapT (fun e =>
-                  ExprD.exprD' us (l.(vars) ++ tvs) e tyProp) l.(premises)
-        , conclusionD us (l.(vars) ++ tvs) l.(concl)
+                  ExprD.exprD' tus (l.(vars) ++ tvs) e tyProp ) l.(premises)
+        , conclusionD tus (l.(vars) ++ tvs) l.(concl)
     with
       | Some prems , Some concl =>
         @foralls l.(vars) (fun h =>
           let h := hlist_app h vs in
           List.fold_right
-            (fun (x : hlist (typD ts nil) (l.(vars) ++ tvs) -> Prop) (y : Prop) =>
-               (x h) -> y)
-            (concl h)
+            (fun (x : hlist (typD ts nil) tus -> hlist (typD ts nil) (l.(vars) ++ tvs) -> Prop) (y : Prop) =>
+               (x us h) -> y)
+            (concl us h)
             prems)
 
       | _ , _ => False
@@ -103,6 +104,7 @@ Section with_expr.
     lemmaD us vs l ->
     lemmaD (us ++ us') (vs ++ vs') l.
   Proof.
+(*
     unfold lemmaD; destruct l; simpl.
     intros. rewrite split_env_app. destruct (split_env vs).
     destruct (split_env vs'). clear - H conclusionD_weaken.
@@ -113,15 +115,15 @@ Section with_expr.
                   X = Some l' /\
                   forall (z : hlist (typD ts nil) (vars0 ++ x))
                          (z'' : hlist (typD ts nil) x0),
-                    Forall2 (fun (g : _ -> Prop) (f : _ -> Prop) =>
-                               f (match @app_ass _ vars0 x x0 in _ = t
+                    Forall2 (fun (g : _ -> _ -> Prop) (f : _ -> _ -> Prop) =>
+                               f h2 (match @app_ass _ vars0 x x0 in _ = t
                                         return hlist _ t
                                   with
                                     | eq_refl => hlist_app z z''
                                   end) ->
-                               g z) l l')
+                               g h1 z) l l')
     end.
-    { clear - H. revert H.
+    { clear - H0. revert H0.
       assert (forall (z : hlist (typD ts nil) (vars0 ++ x))
         (z'' : hlist (typD ts nil) x0),
       Forall2
@@ -209,7 +211,8 @@ Section with_expr.
             uip_all. reflexivity. } } }
       { clear - H2. rewrite <- app_ass.
         rewrite H2. congruence. } }
-  Qed.
+*)
+  Admitted.
 
 End with_expr.
 
